whole thing verifies for memory safety

code/shorthash/Hacl.Impl.Shorthash.SipHash24.fst
@@ -267,7 +267,7 @@ val siphash_aligned:
   datalen :uint32_ht{U32.v datalen = Buffer.length data} ->
   Stack unit
     (requires (fun h -> live h v /\ live h data))
-    (ensures  (fun h0 _ h1 -> live h1 v /\ live h1 data // /\ modifies_1 v h0 h1
+    (ensures  (fun h0 _ h1 -> live h1 v /\ live h1 data /\ modifies_1 v h0 h1
                          /\ (let arg_v = as_seq h0 v in
                             let data_v = as_seq h0 data in
                             let spec_v = Spec.siphash_aligned arg_v data_v in
@@ -359,7 +359,7 @@ val accumulate_unaligned:
                         /\ U32.v i + U32.v len < 8
                         /\ (let (n:nat{n <= 7 /\ (U32.v i) + (Buffer.length buf) == n}) = (U32.v len + U32.v i) in
                            let spec_r = Spec.accumulate_unaligned mi (as_seq h0 buf) i n in
-			   True)))//r == spec_r)))
+			   True))) // r == spec_r)))
 inline_for_extraction
 let rec accumulate_unaligned mi buf i len =
   (**) let h0 = ST.get() in
@@ -385,92 +385,12 @@ let rec accumulate_unaligned mi buf i len =
     let mi'' = accumulate_unaligned mi' buf' (i `U32.add` 1ul) len' in
     (**) let h1 = ST.get() in
     (**) assert(modifies_0 h0 h1);
-    (**) lemma_accumulate_1 mi mi' (as_seq h0 buf') (i `U32.add` 1ul) n;
-    // (**) assert(mi'' == Spec.accumulate_unaligned mi (as_seq h0 buf) i n);
+    // (**) assert(mi'' == Spec.accumulate_unaligned mi' (as_seq h0 buf') (i `U32.add` 1ul) n);
     mi''
   )
 
-(*  
-  else (
-    (**) assert(U32.v datalen > 0);
-
-    let mi = data.(0ul) in
-    siphash_inner v mi;
-
-    (**) let h1 = ST.get() in
-
-    let datalen' = datalen `U32.sub` 1ul in
-    let data' = Buffer.sub data 1ul datalen' in
-
-    (**) let h2 = ST.get() in
-    (**) assert(Buffer.modifies_1 v h0 h1);
-    (**) Buffer.no_upd_lemma_1 h0 h1 v data;
-    (**) Buffer.no_upd_lemma_0 h1 h2 data;
-    (**) assert((as_seq h0 data) = (as_seq h2 data));
-    (**) assert(as_seq h2 data' == Seq.slice (as_seq h2 data) 1 (U32.v datalen));
-    (**) assert(Seq.length (as_seq h2 data') == U32.v datalen');
-
-    siphash_aligned' v data' datalen';
-
-    (**) let h3 = ST.get() in
-    (**) Buffer.no_upd_lemma_1 h2 h3 v data;
-    (**) assert((as_seq h2 data) = (as_seq h3 data));
-    (**) let arg_v = as_seq h0 v in
-    (**) let data_v = as_seq h0 data in
-    (**) let impl_v = as_seq h3 v in
-    (**) assert(mi == Seq.index data_v 0);
-    (**) assert(as_seq h1 v == Spec.siphash_inner (as_seq h0 v) mi);
-    (**) assert(as_seq h1 v == as_seq h2 v);
-    (**) assert(as_seq h2 data' == Seq.slice data_v 1 (Seq.length data_v));
-    (**) assert(as_seq h3 v == Spec.siphash_aligned' (as_seq h2 v) (Seq.slice data_v 1 (Seq.length data_v)))
-  )
-
-
-  (**) let h0 = ST.get() in
-  (**) let inv (h1:HS.mem) (i:nat) : Type0 =
-         i <= Buffer.length buf /\ i < 8
-       /\ live h1 buf /\ live h1 mi /\ modifies_1 mi h0 h1 
-       /\ as_seq h0 buf == as_seq h1 buf
-       /\ (let mi0 = as_uint64 h0 mi in
-          assert(as_seq h0 mi == Seq.create 1 0uL);
-          assert(mi0 == Seq.index (Seq.create 1 0uL) 0);
-          assert(mi0 == 0uL);
-          let arg_buf = as_seq h0 buf in
-          let sliced_buf = Seq.slice arg_buf 0 i in
-	  assert(Seq.length sliced_buf == i);
-          let spec_v = Spec.accumulate_unaligned mi0 sliced_buf 0ul i  in
-          let impl_v = as_uint64 h1 mi in
-	  let _ = lemma_accumulate_0 mi0 sliced_buf i in
-          i == 0 ==> ((Spec.accumulate_unaligned mi0 sliced_buf 0ul i) == mi0)) // (Spec.accumulate_unaligned mi0 sliced_buf 0ul i == mi0)) // impl_v == spec_v)
-       in
-
-  let body (i:uint32_ht {U32.v 0ul <= U32.v i /\ i `U32.lt` len}) :
-    Stack unit
-      (requires (fun h -> inv h (U32.v i)))
-      (ensures  (fun h0 _ h1 -> inv h1 (U32.v i + 1)))
-    = (
-      (**) let hbody = ST.get() in
-      let num8 = buf.(i) in
-      let num = FStar.Int.Cast.uint8_to_uint64 num8 in
-      mi.(0ul) <- mi.(0ul) +%^ (num <<^ (i `U32.mul` 8ul));
-      (**) let ii = U32.v i in
-      (**) let mi0 = as_uint64 h0 mi in
-      (**) let arg_buf = as_seq h0 buf in
-      (**) let sliced_buf = Seq.slice arg_buf 0 (ii + 1) in
-      (**) let spec_v = Spec.accumulate_unaligned mi0 sliced_buf 0ul ii in
-      (**) let snum:uint8_ht = Seq.index sliced_buf (ii) in
-      (**) assert(snum == num8))
-  in
-  for 0ul len inv body;
-  let result = mi.(0ul) in
-
-  (**) pop_frame ();
-  (**) let hfin = ST.get() in
-  result
-*)
 
 #reset-options "--max_fuel 0  --z3rlimit 20"
-(*
 inline_for_extraction
 val get_unaligned:
   buf     :uint8_p ->
@@ -483,8 +403,10 @@ val get_unaligned:
 			  //  r == spec_r)))
 inline_for_extraction
 let get_unaligned buf len datalen =
-  let mi = accumulate_unaligned buf len in
-  mi +%^ ((datalen %^ 256uL) <<^ 56ul)
+  let mi = accumulate_unaligned 0uL buf 0ul len in
+  mi +%^ (((uint32_to_uint64 datalen) %^ 256uL) <<^ 56ul)
+
+#reset-options "--max_fuel 0  --z3rlimit 50"
 
 inline_for_extraction
 val siphash_unaligned:
@@ -492,21 +414,23 @@ val siphash_unaligned:
   data    :uint8_p ->
   datalen :uint32_ht {U32.v datalen = Buffer.length data} ->
   Stack unit
-    (requires (fun h -> live h v /\ live h data))
+    (requires (fun h -> live h v /\ live h data /\ disjoint v data))
     (ensures (fun h0 _ h1 -> live h1 v /\ live h1 data /\ modifies_1 v h0 h1 /\
                           (let spec_v = Spec.siphash_unaligned (as_seq h0 v) (as_seq h0 data) in
                            let impl_v = as_seq h1 v in
-                           impl_v = spec_v)))
+                           True))) // impl_v = spec_v)))
 inline_for_extraction
 let siphash_unaligned v data datalen =
-  let final_off = (datalen `U32.div` 8ul) `U32.mul_mod` 8ul in
+  (**) push_frame ();
+  let final_off = (datalen `U32.div` 8ul) `U32.mul` 8ul in
   let slice_len = datalen `U32.sub` final_off in
-  let final_mi = get_unaligned (Buffer.sub data final_off slice_len) slice_len datalen in
+  let remaining = Buffer.sub data final_off slice_len in
+  let final_mi = get_unaligned remaining slice_len datalen in
 
   siphash_inner v final_mi;
 
-  v.(2ul) <- v.(2ul) ^^ 0xffuL
-
+  v.(2ul) <- v.(2ul) ^^ 0xffuL;
+  (**) pop_frame ()
 
 
 inline_for_extraction
@@ -515,15 +439,17 @@ val siphash_finalize:
   Stack uint64_ht
     (requires (fun h -> live h v))
     (ensures (fun h0 _ h1 -> live h1 v /\ modifies_1 v h0 h1 /\
-                          (let spec_v = Spec.siphash_finalize (as_seq h0 v) in
-                           let impl_v = as_seq h1 v in
-                           impl_v == spec_v)))
+                          (let spec_r = Spec.siphash_finalize (as_seq h0 v) in
+                           True))) // impl_v == spec_v)))
 inline_for_extraction
 let siphash_finalize v =
+  (**) push_frame ();
   v.(2ul) <- v.(2ul) ^^ 0xffuL;
   double_round v;
   double_round v;
-  v.(0ul) ^^ v.(1ul) ^^ v.(2ul) ^^ v.(3ul)
+  let result = v.(0ul) ^^ v.(1ul) ^^ v.(2ul) ^^ v.(3ul) in
+  (**) pop_frame ();
+  result
 
 
 #reset-options "--max_fuel 0  --z3rlimit 25"
@@ -533,16 +459,14 @@ val siphash24:
   key0    :uint64_ht ->
   key1    :uint64_ht ->
   data    :uint8_p ->
-  datalen :uint32_ht {U32.v datalen = length data} ->
+  datalen :uint32_ht {U32.v datalen = Buffer.length data} ->
   Stack uint64_ht
         (requires (fun h -> live h data))
         (ensures  (fun h0 r h1 -> live h1 data /\ live h0 data
                              /\ modifies_0 h0 h1 // data is unmodified
-                             /\ (r == Spec.siphash24 key0 key1 (as_seq h0 data)))) // result matches spec
+                             )) // /\ (r == Spec.siphash24 key0 key1 (as_seq h0 data)))) // result matches spec
 let siphash24 key0 key1 data datalen =
-
   (**) push_frame ();
-  (**) let h0 = ST.get() in
 
   let v = Buffer.create 0uL 4ul in
 
@@ -554,4 +478,3 @@ let siphash24 key0 key1 data datalen =
   (**) pop_frame ();
 
   result
-*)
